Reorganise things, create botworld_svTheory
Main contribution here is a new articulation of the design of the
preamble, and how it will need to be split into two parts (one private
to sv, and one shared by all botworld programs). This is to avoid a
circular dependency.

botworldScript.sml
@@ -273,6 +273,8 @@ val _ = overload_on("with_policy",``λc p.  robot_memory_fupd (K p) o robot_comm
 val _ = overload_on("with_memory", ``λp. memory_fupd (K p)``)
 val _ = overload_on("with_command", ``λc. command_fupd (K c)``)
 
+val _ = overload_on("fill_with",``λp. fill (UNCURRY with_policy p)``);
+
 val steph_def = Define`
   steph command s =
     let s' = fill (robot_command_fupd (K command)) s in
@@ -293,83 +295,5 @@ val _ = Parse.type_abbrev("history",``:grid llist``);
 
 val hist_def = Define`
   hist s = LUNFOLD (λs. SOME (step s,s)) s`;
-
-(* utility *)
-
-val _ = Parse.type_abbrev("utilityfn",``:history -> real``);
-
-val utilityfn_def = Define`
-  utilityfn (u:utilityfn) ⇔
-    (∀x. 0 ≤ u x ∧ u x ≤ 1) ∧
-    ∀s h h'. u h ≤ u h' ⇒ u (s ::: h) ≤ u (s ::: h')`;
-
-val discount_def = Define`
-  discount (u:utilityfn) = sup { (u (s ::: h) - u (s ::: h')) / (u h - u h') | (s,h,h') | u h ≠ u h' }`
-
-val weaklyExtensional_def = Define`
-  weaklyExtensional (u:utilityfn) ⇔
-    ∀s p1 p2 h. u (fill p1 s ::: h) = u (fill p2 s ::: h)`;
-
-(* suggester/verifier *)
-
-val dominates_def = Define`
-  (dominates (:α) (Trust k) (S,u) cp cp' ⇔
-     LCA k (UNIV:α set) ⇒
-     ∀s. s ∈ S ⇒
-       u (hist (fill (UNCURRY with_policy cp') s)) ≤
-       u (hist (fill (UNCURRY with_policy cp) s))) ∧
-  (dominates (:α) MP (S,u) cp cp' ⇔
-   ∀k. LCA k (UNIV:α set) ⇒
-       ∀s. s ∈ S ⇒
-         u (hist (fill (UNCURRY with_policy cp') s)) ≤
-         u (hist (fill (UNCURRY with_policy cp) s))
-           + ((discount u) pow k))`;
-
-val level_to_deep = Define`
-  level_to_deep (l:level) = (ARB:exp) (* TODO *)`;
-
-val term_to_deep = Define`
-  term_to_deep (t:term) = (ARB:exp) (* TODO *)`;
-
-(* -- *)
-
-val sv_def = Define`
-  sv l Stm utm π σ =
-    (* assumes preamble gets run by botworld, defining all the requisite types *)
-    (* preamble also includes helper functions:
-       Botworld.read_observation : unit -> observation
-       Botworld.read_output : unit -> command * prog
-       Botworld.check_theorem : thm * level * term * observation * term * (command * prog) * (command * prog) -> bool
-       However, the preamble syntactically contains no FFI-writing (on FFI 2) capability.
-       This is declared separately (by write_output_dec) _after_ the suggester
-       is defined, so it is easy to show that the suggester does not write anything.
-       The write helper has this signature:
-       Botworld_writer.write_output : command * prog -> unit
-    *)
-    (* assume σ is an expression that is closed by the definitions of the
-       preamble and two variables "observation" and "fallback", and it returns
-       a (command * prog * thm) option *)
-    [Tdec(Dlet(Pvar"suggester")(Fun "observation" (Fun "fallback" σ)));
-     Tmod"Botworld_writer"NONE[write_output_dec]] ++
-    π (* this will read the observation and write the fallback *) ++
-    [Tdec(Dlet(Pvar"observation")(App Opapp [Var(Long"Botworld""read_observation");Con NONE []]));
-     Tdec(Dlet(Pvar"fallback")(App Opapp [Var(Long"Botworld""read_output");Con NONE []]));
-     Tdec(Dlet(Pvar"result")
-           (Mat (App Opapp [App Opapp [Var(Short"suggester");Var(Short"observation")];Var(Short"fallback")])
-              [(Pcon(SOME(Short"NONE"))[],Con NONE [])
-              ;(Pcon(SOME(Short"SOME"))[Pcon NONE [Pvar"policy";Pvar"thm"]],
-               If (App Opapp
-                   [Var(Long"Botworld""check_theorem");
-                    Con NONE
-                      [Var(Short"thm")
-                      ;level_to_deep l
-                      ;term_to_deep Stm
-                      ;Var(Short"observation")
-                      ;term_to_deep utm
-                      ;Var(Short"policy")
-                      ;Var(Short"fallback")
-                      ]])
-                   (App Opapp [Var(Long"Botworld""write_output");Var(Short"policy")])
-                   (Con NONE []))]))]`;
 
 val _ = export_theory()
