botworld_svScript.sml
@@ -1,0 +1,218 @@
+open preamble
+     botworld_quoteTheory
+     basicReflectionLib
+     holKernelTheory
+
+val _ = new_theory"botworld_sv"
+
+val _ = Parse.bring_to_front_overload","{Name=",",Thy="pair"};
+val _ = Parse.hide"S";
+
+(* utility *)
+
+val _ = Parse.type_abbrev("utilityfn",``:history -> real``);
+
+val utilityfn_def = Define`
+  utilityfn (u:utilityfn) ⇔
+    (∀x. 0 ≤ u x ∧ u x ≤ 1) ∧
+    ∀s h h'. u h ≤ u h' ⇒ u (s ::: h) ≤ u (s ::: h')`;
+
+val discount_def = Define`
+  discount (u:utilityfn) = sup { (u (s ::: h) - u (s ::: h')) / (u h - u h') | (s,h,h') | u h ≠ u h' }`
+
+val weaklyExtensional_def = Define`
+  weaklyExtensional (u:utilityfn) ⇔
+    ∀s p1 p2 h. u (fill p1 s ::: h) = u (fill p2 s ::: h)`;
+
+val discount_exists_def = Define`
+  discount_exists (u:utilityfn) ⇔
+    (∃h1 h2. u h1 ≠ u h2) ∧
+    (∃z. ∀s h1 h2. u h1 ≠ u h2 ⇒ (u (s:::h2) − u (s:::h1)) / (u h2 − u h1) < z)`;
+
+val discount_not_negative = Q.store_thm("discount_not_negative",
+  `utilityfn u ∧ discount_exists u ⇒ 0 ≤ discount u`,
+  rw[utilityfn_def,discount_def,discount_exists_def]
+  \\ qmatch_goalsub_abbrev_tac`sup P`
+  \\ `∃x. P x` by ( simp[Abbr`P`,UNCURRY] \\ simp[EXISTS_PROD] \\ metis_tac[])
+  \\ `∃z. ∀x. P x ⇒ x < z`
+  by (
+    simp[Abbr`P`,UNCURRY] \\ simp[EXISTS_PROD]
+    \\ simp[PULL_EXISTS] \\ metis_tac[] )
+  \\ `∃x. P x ∧ 0 ≤ x` suffices_by metis_tac[realTheory.REAL_SUP_UBOUND,realTheory.REAL_LE_TRANS]
+  \\ simp[Abbr`P`,UNCURRY,EXISTS_PROD]
+  \\ simp[PULL_EXISTS]
+  \\ asm_exists_tac \\ simp[]
+  \\ Cases_on`u h2 ≤ u h1`
+  >- (
+    last_x_assum drule
+    \\ disch_then(qspec_then`s`strip_assume_tac)
+    \\ qexists_tac`s`
+    \\ match_mp_tac realTheory.REAL_LE_DIV
+    \\ simp[realTheory.REAL_SUB_LE] )
+  \\ pop_assum mp_tac
+  \\ simp[realTheory.REAL_NOT_LE,realTheory.REAL_LT_LE]
+  \\ strip_tac
+  \\ last_x_assum drule
+  \\ disch_then(qspec_then`s`strip_assume_tac)
+  \\ qexists_tac`s`
+  \\ ONCE_REWRITE_TAC [GSYM realTheory.REAL_NEG_LE0]
+  \\ ONCE_REWRITE_TAC [realTheory.neg_rat]
+  \\ IF_CASES_TAC >- metis_tac[realTheory.REAL_SUB_0]
+  \\ simp[realTheory.REAL_NEG_SUB]
+  \\ qmatch_abbrev_tac`a / b ≤ 0`
+  \\ `0 ≤ a / -b`
+  suffices_by (
+    REWRITE_TAC[realTheory.neg_rat]
+    \\ IF_CASES_TAC >- metis_tac[realTheory.REAL_SUB_0]
+    \\ ONCE_REWRITE_TAC[GSYM realTheory.REAL_NEG_LE0]
+    \\ REWRITE_TAC[realTheory.neg_rat]
+    \\ IF_CASES_TAC >- metis_tac[realTheory.REAL_SUB_0]
+    \\ simp[] )
+  \\ simp[realTheory.REAL_NEG_SUB,Abbr`a`,Abbr`b`]
+  \\ match_mp_tac realTheory.REAL_LE_DIV
+  \\ simp[realTheory.REAL_SUB_LE] );
+
+(* suggester/verifier *)
+
+val dominates_def = Define`
+  (dominates (:α) (Trust k) (S,u) cp cp' ⇔
+     LCA k (UNIV:α set) ⇒
+     ∀s. s ∈ S ⇒
+       u (hist (fill (UNCURRY with_policy cp') s)) ≤
+       u (hist (fill (UNCURRY with_policy cp) s))) ∧
+  (dominates (:α) MP (S,u) cp cp' ⇔
+   ∀k. LCA k (UNIV:α set) ⇒
+       ∀s. s ∈ S ⇒
+         u (hist (fill (UNCURRY with_policy cp') s)) ≤
+         u (hist (fill (UNCURRY with_policy cp) s))
+           + ((discount u) pow k))`;
+
+val dominates_refl = Q.store_thm("dominates_refl",
+  `utilityfn u ∧ discount_exists u ⇒ dominates a l (S,u) cp cp`,
+  Cases_on`a`\\Cases_on`l`\\simp[dominates_def]
+  \\ simp[realTheory.REAL_LE_ADDR]
+  \\ metis_tac[discount_not_negative,realTheory.POW_POS]);
+
+val dominates'_def = Define`
+  (dominates' a (Trust k) g cp cp' = dominates a (Trust (SUC k)) g cp cp') ∧
+  (dominates' (:α) MP (S,u) cp cp' =
+   ∀k. LCA (SUC k) 𝕌(:α) ⇒ ∀s. s ∈ S ⇒
+     u (hist (fill_with cp' s)) ≤ u (hist (fill_with cp s)) + (discount u) pow k)`;
+
+val dominates'_refl = Q.store_thm("dominates'_refl",
+  `utilityfn u ∧ discount_exists u ⇒ dominates' a l (S,u) cp cp`,
+  Cases_on`a`\\reverse(Cases_on`l`)\\simp[dominates'_def]
+  >- metis_tac[dominates_refl]
+  \\ simp[realTheory.REAL_LE_ADDR]
+  \\ metis_tac[discount_not_negative,realTheory.POW_POS]);
+
+val level_to_deep_def = Define`
+  level_to_deep (l:level) = (ARB:exp) (* TODO *)`;
+
+val term_to_deep_def = Define`
+  (* term_to_deep (Var s ty) = App Opapp [Var(Long"Botworld""mk_var"); Con NONE [Lit (StrLit (explode s)); type_to_deep ty]] ∧ *)
+  term_to_deep (t:term) = (ARB:exp) (* TODO *)`;
+
+(* -- *)
+
+val _ = overload_on("state_with_hole_ty",type_to_deep``:state_with_hole``);
+val _ = overload_on("observation_ty",type_to_deep``:observation``);
+val _ = overload_on("utilityfn_ty",type_to_deep``:utilityfn``);
+val _ = overload_on("dominates_tm",term_to_deep``dominates (:α)``);
+
+val mk_target_concl_def = Define`
+  mk_target_concl obs cp1 cp2 l Stm utm =
+  Comb
+  (Comb
+   (Comb
+    (Comb dominates_tm (FST quote_level l))
+    (FST (quote_prod
+          ((I, Fun state_with_hole_ty Bool), (I, utilityfn_ty)))
+     (Comb Stm (FST quote_observation obs), utm)))
+   (FST (quote_prod (quote_command, quote_prog)) cp1))
+  (FST (quote_prod (quote_command, quote_prog)) cp2)`;
+
+val check_theorem_def = Define`
+  check_theorem thm l Stm obs utm cp1 cp2 =
+    aconv (concl thm) (mk_target_concl obs cp1 cp2 l Stm utm)`;
+
+(* TODO: translate mk_target_concl *)
+
+(*
+val sv_body_def = Define`
+  sv_body l Stm utm σ obs cp1 =
+   case σ obs cp1 of
+   | NONE => NONE
+   | SOME (cp2,th) =>
+       if aconv (concl th) (mk_target_concl obs cp1 cp2 l Stm utm)
+*)
+
+(* Two preambles.
+   1. Botworld preamble, at the end of which we have preamble_env, which is
+      called by run_policy.
+   2. sv_preamble, which is all the rest of the preamble stuff and only sv has
+      access to it.
+
+  Botworld preamble:
+    - Pure library functions:
+      - Pure cores of I/O functions
+      - Botworld datatype
+      - CakeML datatypes
+    - Candle kernel functions:
+      - the monadic functions in holKernelTheory
+    - Impure I/O wrappers
+      - read/write functions that call FFI
+
+  sv_preamble:
+    - Candle definitions of botworld, up to dominates
+      - i.e., build the inner_ctxt
+      - N.B.: this includes defining preamble_env
+    - definition of check_theorem
+*)
+
+val sv_def = Define`
+  sv l Stm utm π σ =
+    (* assumes Botworld preamble gets run by botworld *)
+    (* Botworld preamble includes helper functions:
+       Botworld.read_observation : unit -> observation
+       Botworld.read_output : unit -> command * prog
+       Botworld.write_output : command * prog -> unit
+    *)
+    (*
+       sv_preamble includes:
+       check_theorem : thm * level * term * observation * term * (command * prog) * (command * prog) -> bool
+    *)
+    (*
+      N.B. The only functions in either preamble that call any FFI are
+           Botworld.read_observation,
+           Botworld.read_output,
+           Botworld.write_output
+    *)
+    (*
+      Assume σ is an expression that is closed by the definitions of the both
+      preambles, not including the FFI-calling functions, and two variables
+      "observation" and "fallback", and it returns a (command * prog * thm) option
+    *)
+    π (* this will read the observation and write the fallback *) ++
+    (* TODO: insert sv_preamble here *)
+    [Tdec(Dlet(Pvar"observation")(App Opapp [Var(Long"Botworld""read_observation");Con NONE []]));
+     Tdec(Dlet(Pvar"fallback")(App Opapp [Var(Long"Botworld""read_output");Con NONE []]));
+     Tdec(Dlet(Pvar"result")
+           (Mat σ (* n.b. σ refers to the observation and fallback variables *)
+              [(Pcon(SOME(Short"NONE"))[],Con NONE [])
+              ;(Pcon(SOME(Short"SOME"))[Pcon NONE [Pvar"policy";Pvar"thm"]],
+               If (App Opapp
+                   [Var(Long"Botworld""check_theorem");
+                    Con NONE
+                      [Var(Short"thm")
+                      ;level_to_deep l
+                      ;term_to_deep Stm
+                      ;Var(Short"observation")
+                      ;term_to_deep utm
+                      ;Var(Short"policy")
+                      ;Var(Short"fallback")
+                      ]])
+                   (App Opapp [Var(Long"Botworld""write_output");Var(Short"policy")])
+                   (Con NONE []))]))]`;
+
+val _ = export_theory()
